merge L0.thy and LD_Issues.thy

papers/116_stefan_rass/L0.thy
@@ -70,65 +70,6 @@ proof -
   qed
 qed
 
-lemma T_superlinear: "\<forall>N. \<exists>n\<^sub>0. \<forall>n\<ge>n\<^sub>0. T(n)/n \<ge> N"
-proof (intro allI)
-  fix N :: real
-
-  show "\<exists>n\<^sub>0. \<forall>n\<ge>n\<^sub>0. T(n)/n \<ge> N"
-  proof (cases "N > 0")
-    assume "\<not> N > 0"
-    then have "N \<le> 0" by simp
-    also have "0 \<le> T(n)/n" for n by simp
-    finally show ?thesis by simp
-  next
-    assume "N > 0"
-    then have *: "N \<le> N * x" if "x \<ge> 1" for x
-      using that by (subst mult_le_cancel_left1) simp
-
-    from T_ge_t_log_t_ae[of 1] have "ae n. t n * log 2 (t n) < T n" unfolding mult_1 by argo
-    with t_min have "ae n. T(n)/n \<ge> N"
-    proof (ae_intro_nat)
-      fix n :: nat
-      assume "n \<ge> 2 ^ nat\<lceil>N\<rceil>" and t_log_t: "t n * log 2 (t n) < T n"
-
-      from two_realpow_ge_one have "(1::real) \<le> 2 ^ nat\<lceil>N\<rceil>" .
-      also from \<open>n \<ge> 2 ^ nat\<lceil>N\<rceil>\<close> have "... \<le> n" by simp
-      finally have "n > 0" by simp
-
-      also assume "n \<le> t n"
-      finally have "t n > 0" .
-
-
-      have "n * log 2 n \<le> t n * log 2 (t n)"
-      proof (intro mult_mono)
-        from \<open>n \<le> t n\<close> show "real n \<le> real (t n)" by simp
-        with \<open>n > 0\<close> and \<open>t n > 0\<close> show "log 2 n \<le> log 2 (t n)"
-          by (subst log_le_cancel_iff; linarith)
-
-        show "real (t n) \<ge> 0" by (fact of_nat_0_le_iff)
-        from \<open>n > 0\<close> show "0 \<le> log 2 (real n)"
-          by (subst zero_le_log_cancel_iff) auto
-      qed
-      also from t_log_t have "... < T n" .
-      finally have "n * log 2 n \<le> T n" by simp
-
-      with \<open>n > 0\<close> have "log 2 n \<le> T(n)/n" by (subst pos_le_divide_eq) (simp, argo)
-
-      have "N \<le> log 2 n"
-      proof -
-        have "N \<le> log 2 (2 ^ nat\<lceil>N\<rceil>)"
-          by (subst log_pow_cancel) (simp, simp, linarith)
-        also have "... \<le> log 2 n" using \<open>n \<ge> 2 ^ nat\<lceil>N\<rceil>\<close> and \<open>n > 0\<close>
-          by (subst log_le_cancel_iff) auto
-        finally show "N \<le> log 2 n" .
-      qed
-      also note \<open>log 2 n \<le> T(n)/n\<close>
-      finally show "N \<le> T(n)/n" .
-    qed
-    then show "\<exists>n\<^sub>0. \<forall>n\<ge>n\<^sub>0. T(n)/n \<ge> N" ..
-  qed
-qed
-
 
 text\<open>\<open>L\<^sub>D\<close>, defined as part of the proof for the Time Hierarchy Theorem.
 
@@ -221,11 +162,89 @@ theorem time_hierarchy: "L\<^sub>D \<in> DTIME(T) - DTIME(t)" using LD_T and LD_
 end \<comment> \<open>\<^locale>\<open>tht_assms\<close>\<close>
 
 
-subsection\<open>The Hard Language \<open>L\<^sub>0\<close>\<close>
+subsection\<open>The Intermediate Language \<open>L\<^sub>D''\<close>\<close>
+
+subsubsection\<open>Encoding\<close>
+
+text\<open>Decode a pair of \<open>(l, x) \<in> \<nat> \<times> {0,1}*\<close> from its encoded form \<open>w \<in> {0,1}*\<close>.
+
+  The encoding defined by this should have \<open>l\<close> encoded in the upper (more significant) bits of \<open>l\<parallel>x\<close>.
+
+  \<open>w\<close> is related to \<open>(l, x)\<close> through the regular expression \<open>1\<^sup>l0x{0,1}\<^sup>k\<close>,
+  where \<^term>\<open>k = suffix_len w\<close>.
+  If \<open>w\<close> does not match the expression, default values \<open>l = 0, x = []\<close> are assigned.
+
+  Construction:
+  To ensure the required property for Lemma 4.6@{cite rassOwf2017}, the lower half of \<open>w\<close>
+  (the \<open>k\<close> least-significant-bits) is dropped.
+  Then, \<open>l\<close> is the number of leading \<open>1\<close>s.
+  Remove all leading \<open>1\<close>s and one \<open>0\<close> to retain \<open>x\<close>.\<close>
+
+definition strip_sq_pad :: "word \<Rightarrow> word"
+  where "strip_sq_pad w \<equiv> drop (suffix_len w) w"
+definition decode_pair_l :: "word \<Rightarrow> nat"
+  where "decode_pair_l w = length (takeWhile (\<lambda>x. x = True) (rev (strip_sq_pad w)))"
+definition decode_pair_x :: "word \<Rightarrow> word"
+  where "decode_pair_x w = rev (tl (dropWhile (\<lambda>x. x = True) (rev (strip_sq_pad w))))"
+abbreviation decode_pair :: "word \<Rightarrow> nat \<times> word"
+  where "decode_pair w \<equiv> (decode_pair_l w, decode_pair_x w)"
+
+definition rev_suffix_len :: "word \<Rightarrow> nat"
+  where "rev_suffix_len w = length w + 9"
+definition encode_pair :: "nat \<Rightarrow> word \<Rightarrow> word"
+  where "encode_pair l x = (let w' = x @ [False] @ True \<up> l in
+            False \<up> (rev_suffix_len w') @ w')"
+
+lemma encode_pair_altdef:
+  "encode_pair l x = False \<up> (length x + l + 10) @ x @ [False] @ True \<up> l"
+  unfolding encode_pair_def rev_suffix_len_def Let_def by simp
+
+lemma strip_sq_pad_pair:
+  fixes l x
+  defines w: "w \<equiv> encode_pair l x"
+    and w': "w' \<equiv> x @ [False] @ True \<up> l"
+  shows "strip_sq_pad w = w'"
+proof -
+  let ?lw = "length w" and ?lw' = "length w'"
+  have lw: "?lw = 2 * ?lw' + 9" unfolding w w' encode_pair_altdef by simp
+  have lwh: "5 + ?lw div 2 = rev_suffix_len w'" unfolding lw rev_suffix_len_def by simp
+  show "strip_sq_pad w = w'" unfolding strip_sq_pad_def suffix_len_def lwh
+    unfolding w encode_pair_def Let_def w'[symmetric] by simp
+qed
+
+lemma decode_encode_pair:
+  fixes l x
+  defines w: "w \<equiv> encode_pair l x"
+  shows "decode_pair w = (l, x)"
+proof (unfold prod.inject, intro conjI)
+  have rw: "rev (strip_sq_pad w) = True \<up> l @ False # rev x" unfolding w strip_sq_pad_pair by force
+  show "decode_pair_l w = l" unfolding decode_pair_l_def rw by (subst takeWhile_tail) auto
+  show "decode_pair_x w = x" unfolding decode_pair_x_def rw by (subst dropWhile_append3) auto
+qed
 
 
-lemma SQ_DTIME: "SQ \<in> DTIME(\<lambda>n. n^3)" sorry
+lemma pair_adj_sq_eq:
+  fixes w
+  defines w': "w' \<equiv> adj_sq\<^sub>w w"
+  assumes len: "length w \<ge> 9"
+  shows "decode_pair w' = decode_pair w"
+proof -
+  let ?sl = "suffix_len w" and ?lw = "length w" and ?lw' = "length w'"
+  from len have sh: "shared_MSBs (?lw - ?sl) w w'" unfolding w' by (rule adj_sq_sh_pfx_half)
+  from sh have l_eq: "?lw' = ?lw" ..
 
+  from len have "?sl \<le> length w" by (rule suffix_min_len)
+  then have "?lw - (?lw - ?sl) = ?sl" by (rule diff_diff_cancel)
+  from sh have "drop (?lw' - (?lw - ?sl)) w' = drop (?lw - (?lw - ?sl)) w" ..
+  then have "drop ?sl w' = drop ?sl w" unfolding l_eq \<open>?lw - (?lw - ?sl) = ?sl\<close> .
+  then have sq_pad_eq: "strip_sq_pad w' = strip_sq_pad w"
+    unfolding strip_sq_pad_def suffix_len_def l_eq .
+  show "decode_pair w' = decode_pair w"
+    unfolding decode_pair_x_def decode_pair_l_def sq_pad_eq ..
+qed
+
+
+subsubsection\<open>Definition\<close>
 
 text\<open>From the proof of Lemma 4.6@{cite rassOwf2017}:
 
@@ -234,15 +253,68 @@ text\<open>From the proof of Lemma 4.6@{cite rassOwf2017}:
     to our hypothesis besides Assumption 4.4 (note that we do not need an optimal
     complexity bound here).''\<close>
 
-locale tht_sq_assms = tht_assms +
-  assumes t_cubic: "ae n. t(n) \<ge> n^3"
+locale lemma4_6 =
+  fixes T t l\<^sub>R :: "nat \<Rightarrow> nat"
+  defines "l\<^sub>R \<equiv> \<lambda>n. 4 * n + 11"
+  assumes T_dominates_t': "(\<lambda>n. (t \<circ> l\<^sub>R) n * log 2 ((t \<circ> l\<^sub>R) n) / T n) \<longlonglongrightarrow> 0"
     and t_mono: "mono t"
+    and t_cubic: "ae n. t(n) \<ge> n^3"
+    and tht_assms: "tht_assms T t" (* TODO inline when finalized *)
 begin
 
-corollary T_cubic: "ae n. T(n) \<ge> n^3"
-  by (ae_intro_nat add: t_cubic T_gt_t_ae) linarith
+lemma t'_ge_t: "t n \<le> (t \<circ> l\<^sub>R) n" unfolding l\<^sub>R_def comp_def
+  using t_mono by (elim monoD) linarith
 
-corollary t_superlinear: "\<forall>N. \<exists>n\<^sub>0. \<forall>n\<ge>n\<^sub>0. t(n)/n \<ge> N"
+(* TODO document this approach *)
+
+sublocale tht: tht_assms T "t \<circ> l\<^sub>R"
+  using tht_assms and T_dominates_t'
+proof (unfold tht_assms_def, elim conjE, intro conjI)
+  assume "ae n. n \<le> t n"
+  thus "ae n. n \<le> (t \<circ> l\<^sub>R) n"
+  proof (ae_intro_nat)
+    fix n assume "n \<le> t n"
+    also note t'_ge_t
+    finally show "n \<le> (t \<circ> l\<^sub>R) n" .
+  qed
+qed
+
+
+text\<open>Note: this is not intended to replace \<^const>\<open>tht.L\<^sub>D\<close>.
+  Instead, the further proof uses the similarity of \<open>L\<^sub>D\<close> and \<open>L\<^sub>D''\<close>
+  to prove properties of \<open>L\<^sub>D''\<close> via reduction to \<open>L\<^sub>D\<close>.
+
+  Construction: Given a word \<open>w\<close>.
+  Split the word \<open>w\<close> into \<open>(l::nat, x::word)\<close> using \<^const>\<open>decode_pair\<close>.
+  Define \<open>v\<close> as the \<open>l\<close> most-significant-bits of \<open>x\<close>.
+  Remove the arbitrary-length \<open>1\<^sup>+0\<close>-prefix from \<open>v\<close> to retain the pure encoding of \<open>M\<^sub>v\<close>.
+  If \<open>M\<^sub>v\<close> rejects \<open>v\<close> within \<open>T(len(x))\<close> steps, \<open>w \<in> L\<^sub>D''\<close> holds.
+
+  Note that in this version, using \<^const>\<open>time_bounded_word\<close> is not possible,
+  as the word that determines the time bound (\<open>x\<close>) differs from the input word (\<open>v\<close>).
+  For simplicity, a predicate similar to the shorter but equivalent
+  term for \<^const>\<open>time_bounded_word\<close> is used (@{thm time_bounded_altdef}).\<close>
+
+definition L\<^sub>D'' :: lang
+  where "L\<^sub>D'' \<equiv> {w.
+      let (l, x) = decode_pair w;
+          v = drop (length x - l) x;
+          M\<^sub>v = TM_decode_pad v in
+      rejects M\<^sub>v v \<and> is_final (steps0 (1, <v>\<^sub>t\<^sub>p) M\<^sub>v (tcomp\<^sub>w T x))
+    }"
+
+
+subsubsection\<open>Preliminaries\<close>
+
+lemma T_cubic: "ae n. T(n) \<ge> n^3"
+proof (ae_intro_nat add: t_cubic tht.T_gt_t_ae)
+  fix n assume "n^3 \<le> t n"
+  also from t'_ge_t have "... \<le> (t \<circ> l\<^sub>R) n" .
+  also assume "... < T n"
+  finally show "T(n) \<ge> n^3" by (fact order_less_imp_le)
+qed
+
+lemma t_superlinear: "\<forall>N. \<exists>n\<^sub>0. \<forall>n\<ge>n\<^sub>0. t(n)/n \<ge> N"
 proof (intro allI, ae_intro_nat add: t_cubic)
   fix N :: real and n :: nat
   assume n_min: "n \<ge> max 1 (nat \<lceil>N\<rceil>)" and "t(n) \<ge> n^3"
@@ -261,30 +333,237 @@ proof (intro allI, ae_intro_nat add: t_cubic)
   finally show "t(n)/n \<ge> N" .
 qed
 
-lemma adj_sq_exp_pad:
-  fixes w
-  defines l: "l \<equiv> length w"
-    and w': "w' \<equiv> adj_sq\<^sub>w w"
-  assumes "l \<ge> 20"
-  shows "strip_exp_pad w' = strip_exp_pad w"
-proof -
-  from \<open>l \<ge> 20\<close> have "shared_MSBs (clog l) w w'" unfolding l w' by (rule adj_sq_sh_pfx_log)
-  then have l_eq: "length w' = l" and d_eq: "drop (l - clog l) w' = drop (l - clog l) w"
-    unfolding l by blast+
 
-  have "strip_exp_pad w' = drop (l - clog l) w'" unfolding strip_exp_pad_def l_eq Let_def ..
-  also have "... = drop (l - clog l) w" using d_eq .
-  also have "... = strip_exp_pad w" unfolding strip_exp_pad_def l Let_def ..
+subsubsection\<open>\<open>L\<^sub>D'' \<notin> DTIME(t)\<close> via Reduction from \<open>L\<^sub>D\<close> to \<open>L\<^sub>D''\<close>\<close>
+
+text\<open>Reduce \<open>L\<^sub>D\<close> to \<open>L\<^sub>D''\<close>:
+    Given a word \<open>w\<close>, construct its counterpart \<open>w' := 1\<^sup>l0x0\<^sup>l\<^sup>+\<^sup>9\<close>, where \<open>l = length w\<close>.
+    Decoding \<open>w'\<close> then yields \<open>(l, w)\<close> which results in the intermediate value \<open>v\<close>
+    being equal to \<open>w\<close> in the definition of \<^const>\<open>L\<^sub>D''\<close>.\<close>
+
+definition reduce_LD_LD'' :: "word \<Rightarrow> word"
+  where "reduce_LD_LD'' w \<equiv> encode_pair (length w) w"
+
+lemma reduce_LD_LD''_len: "length (reduce_LD_LD'' w) = 4 * length w + 11"
+  unfolding reduce_LD_LD''_def encode_pair_def rev_suffix_len_def by auto
+
+lemma reduce_LD_LD''_correct:
+  fixes w
+  defines w'': "w'' \<equiv> reduce_LD_LD'' w"
+  shows "w'' \<in> L\<^sub>D'' \<longleftrightarrow> w \<in> tht.L\<^sub>D"
+proof -
+  let ?M\<^sub>w = "TM_decode_pad w"
+  have "w'' \<in> L\<^sub>D'' \<longleftrightarrow> rejects ?M\<^sub>w w \<and> time_bounded_word T ?M\<^sub>w w"
+    unfolding L\<^sub>D''_def w'' reduce_LD_LD''_def mem_Collect_eq decode_encode_pair
+    unfolding diff_self_eq_0 drop_0 Let_def prod.case unfolding time_bounded_altdef ..
+  also have "... \<longleftrightarrow> w \<in> tht.L\<^sub>D" unfolding tht.LD_def mem_Collect_eq Let_def ..
   finally show ?thesis .
 qed
 
-corollary adj_sq_TM_dec:
-  fixes w
-  assumes "length w \<ge> 20"
-  defines "w' \<equiv> adj_sq\<^sub>w w"
-  shows "TM_decode_pad w' = TM_decode_pad w"
-  unfolding TM_decode_pad_def w'_def using \<open>length w \<ge> 20\<close> by (subst adj_sq_exp_pad) fast+
 
-end \<comment> \<open>\<^locale>\<open>tht_sq_assms\<close>\<close>
+lemma L\<^sub>D''_t: "L\<^sub>D'' \<notin> DTIME(t)"
+proof (rule ccontr, unfold not_not)
+  let ?f\<^sub>R = reduce_LD_LD''
+
+  assume "L\<^sub>D'' \<in> DTIME(t)"
+  then have "tht.L\<^sub>D \<in> DTIME(t \<circ> l\<^sub>R)" unfolding comp_def
+  proof (rule reduce_DTIME')
+    show "ae w. (?f\<^sub>R w \<in> L\<^sub>D'' \<longleftrightarrow> w \<in> tht.L\<^sub>D) \<and> (length (?f\<^sub>R w) \<le> l\<^sub>R (length w))"
+    proof (intro ae_conjI ae_everyI)
+      fix w
+      from reduce_LD_LD''_correct show "?f\<^sub>R w \<in> L\<^sub>D'' \<longleftrightarrow> w \<in> tht.L\<^sub>D" .
+      from reduce_LD_LD''_len show "length (?f\<^sub>R w) \<le> l\<^sub>R (length w)" unfolding l\<^sub>R_def by simp
+    qed
+
+    from t'_ge_t show "ae x. real (t x) \<le> real (t (l\<^sub>R x))"
+      unfolding comp_def by (intro ae_everyI of_nat_mono)
+
+    show "\<forall>N. \<exists>n\<^sub>0. \<forall>n\<ge>n\<^sub>0. t(n)/n \<ge> N" by (fact t_superlinear)
+
+    show "computable_in_time t reduce_LD_LD''" sorry \<comment> \<open>Assume that \<^const>\<open>reduce_LD_LD''\<close> can be computed in time \<open>O(n)\<close>.\<close>
+  qed
+
+  moreover from tht.time_hierarchy have "tht.L\<^sub>D \<notin> DTIME(t \<circ> l\<^sub>R)" ..
+  ultimately show False by contradiction
+qed
+
+
+subsubsection\<open>\<open>L\<^sub>D'' \<in> DTIME(T)\<close> via Reduction from \<open>L\<^sub>D''\<close> to \<open>L\<^sub>D\<close>\<close>
+
+lemma L\<^sub>D''_T: "L\<^sub>D'' \<in> DTIME(T)"
+proof -
+  \<comment> \<open>For now this is a carbon copy of the ``proof'' of this part of the THT (@{thm tht.time_hierarchy}).
+
+    Ideally, if the TM constructed in the THT is feasible to construct in Isabelle/HOL,
+    and its properties can be proven, the ``difficult parts'' could potentially be reused.
+    It may suffice to add a pre-processing step for decoding the input word \<open>w\<close> into \<open>x, v\<close>,
+    with \<open>v\<close> being the input for the universal TM part, and \<open>x\<close> the input for the stopwatch.
+
+    Note: it seems feasible to construct this adapter and (if this approach works)
+    reduce the \<open>sorry\<close> statements in the THT and this prove into one common assumption;
+    the existence of the UTM with only \<open>log\<close> time overhead.
+    However, such a construction is not sensible for the current TM model,
+    as multiple tapes and arbitrary alphabets would be necessary required.\<close>
+
+  define L\<^sub>D''_P where "L\<^sub>D''_P \<equiv> \<lambda>w. let (l, x) = decode_pair w;
+          v = drop (length x - l) x;
+          M\<^sub>v = TM_decode_pad v in
+      rejects M\<^sub>v v \<and> is_final (steps0 (1, <v>\<^sub>t\<^sub>p) M\<^sub>v (tcomp\<^sub>w T x))"
+
+  obtain M where "time_bounded T M"
+    and *: "\<And>w. if L\<^sub>D''_P w then accepts M w else rejects M w" sorry (* probably out of scope *)
+  have "decides M L\<^sub>D''" unfolding decides_altdef4
+    unfolding L\<^sub>D''_def mem_Collect_eq L\<^sub>D''_P_def[symmetric] using * ..
+  with \<open>time_bounded T M\<close> show "L\<^sub>D'' \<in> DTIME(T)" by blast
+qed
+
+
+subsection\<open>The Hard Language \<open>L\<^sub>0\<close>\<close>
+
+text\<open>``\<^bold>\<open>Lemma 4.6.\<close> Let \<open>t\<close>, \<open>T\<close> be as in Assumption 4.4 and assume \<open>T(n) \<ge> n\<^sup>3\<close>.
+  Then, there exists a language \<open>L\<^sub>0 \<in> DTIME(T) - DTIME(t)\<close> for which \<open>dens\<^sub>L\<^sub>0(x) \<le> \<surd>x\<close>.''\<close>
+
+definition L\<^sub>0'' :: lang
+  where "L\<^sub>0'' \<equiv> L\<^sub>D'' \<inter> SQ"
+
+
+lemma L\<^sub>D''_adj_sq_iff:
+  fixes w
+  defines w': "w' \<equiv> adj_sq\<^sub>w w"
+  assumes len: "length w \<ge> 9"
+  shows "w' \<in> L\<^sub>D'' \<longleftrightarrow> w \<in> L\<^sub>D''"
+  unfolding L\<^sub>D''_def mem_Collect_eq w' len[THEN pair_adj_sq_eq] ..
+
+lemma L\<^sub>D''_L\<^sub>0''_adj_sq_iff:
+  fixes w
+  defines w': "w' \<equiv> adj_sq\<^sub>w w"
+  assumes len: "length w \<ge> 9"
+  shows "w' \<in> L\<^sub>0'' \<longleftrightarrow> w \<in> L\<^sub>D''"
+  unfolding L\<^sub>0''_def w' using len[THEN L\<^sub>D''_adj_sq_iff] adj_sq_word_correct by blast
+
+lemma L0''_t: "L\<^sub>0'' \<notin> DTIME(t)"
+proof (rule ccontr, unfold not_not)
+  assume "L\<^sub>0'' \<in> DTIME(t)"
+  then have "L\<^sub>D'' \<in> DTIME(t)"
+  proof (rule reduce_DTIME)
+    show "almost_everywhere (\<lambda>w. (adj_sq\<^sub>w w \<in> L\<^sub>0'') = (w \<in> L\<^sub>D'') \<and> length (adj_sq\<^sub>w w) \<le> length w)"
+    proof (intro ae_word_lengthI exI allI impI conjI)
+      fix w :: word assume len: "length w \<ge> 9"
+      from len show "adj_sq\<^sub>w w \<in> L\<^sub>0'' \<longleftrightarrow> w \<in> L\<^sub>D''" by (fact L\<^sub>D''_L\<^sub>0''_adj_sq_iff)
+      from len show "length (adj_sq\<^sub>w w) \<le> length w"
+        by (intro eq_imp_le sh_msbD) (fact adj_sq_sh_pfx_half)
+    qed
+
+    show "\<forall>N. \<exists>n\<^sub>0. \<forall>n\<ge>n\<^sub>0. t(n)/n \<ge> N" by (fact t_superlinear)
+
+    show "computable_in_time t adj_sq\<^sub>w" sorry \<comment> \<open>Assume that \<^const>\<open>adj_sq\<^sub>w\<close> can be computed in time \<open>O(t(n))\<close>.\<close>
+  qed
+
+  moreover have "L\<^sub>D'' \<notin> DTIME(t)" by (fact L\<^sub>D''_t)
+  ultimately show False by contradiction
+qed
+
+
+lemma SQ_DTIME: "SQ \<in> DTIME(\<lambda>n. n^3)" sorry
+
+lemma L0''_T: "L\<^sub>0'' \<in> DTIME(T)"
+proof -
+  let ?T' = "\<lambda>n. real (max (T n) (n^3))"
+  from T_cubic obtain n\<^sub>0 where *: "T(n) \<ge> n^3" if "n \<ge> n\<^sub>0" for n by blast
+
+  from L\<^sub>D''_T and SQ_DTIME have "L\<^sub>0'' \<in> DTIME(?T')"
+    unfolding L\<^sub>0''_def of_nat_max by (rule DTIME_int)
+  then show "L\<^sub>0'' \<in> DTIME(T)"
+  proof (rule DTIME_mono_ae)
+    fix n assume "n \<ge> n\<^sub>0"
+    with * have "T(n) \<ge> n^3" .
+    then show "T n \<ge> ?T' n" by simp
+  qed
+qed
+
+
+theorem L0''_time_hierarchy: "L\<^sub>0'' \<in> DTIME(T) - DTIME(t)" using L0''_T L0''_t ..
+
+theorem dens_L0'': "dens L\<^sub>0'' n \<le> dsqrt n"
+proof -
+  have "dens L\<^sub>0'' n = dens (L\<^sub>D'' \<inter> SQ) n" unfolding L\<^sub>0''_def ..
+  also have "... \<le> dens SQ n" by (subst Int_commute) (rule dens_intersect_le)
+  also have "... = dsqrt n" by (rule dens_SQ)
+  finally show ?thesis .
+qed
+
+lemmas lemma4_6'' = L0''_time_hierarchy dens_L0''
+
+end \<comment> \<open>context \<^locale>\<open>lemma4_6\<close>\<close>
+
+
+lemma lemma4_6:
+  fixes T t :: "nat \<Rightarrow> nat"
+  defines "l\<^sub>R \<equiv> \<lambda>n. 4 * n + 11"
+  defines "t' \<equiv> t \<circ> l\<^sub>R"
+  assumes "fully_tconstr T"
+    and T_dominates_t': "(\<lambda>n. t' n * log 2 (t' n) / T n) \<longlonglongrightarrow> 0"
+    and T_not_0: "ae n. T n \<noteq> 0"
+    and t_cubic: "ae n. t n \<ge> n^3"
+    and "mono t"
+  defines "L\<^sub>0 \<equiv> lemma4_6.L\<^sub>0'' T"
+  shows "L\<^sub>0 \<in> DTIME(T) - DTIME(t)" and "dens L\<^sub>0 n \<le> dsqrt n"
+proof -
+  let ?t' = "t \<circ> (\<lambda>n. 4 * n + 11)"
+
+  have "lemma4_6 T t"
+  proof (unfold_locales)
+    show "(\<lambda>n. ?t' n * log 2 (?t' n) / T n) \<longlonglongrightarrow> 0" by (fold t'_def l\<^sub>R_def) fact
+    show "mono t"
+      and "fully_tconstr T"
+      and "ae n. T n \<noteq> 0"
+      and "ae n. t n \<ge> n^3"
+      by fact+
+
+    from \<open>ae n. t n \<ge> n^3\<close> show t_min: "ae n. t n \<ge> n"
+    proof (ae_intro_nat)
+      fix n :: nat
+      have "n \<le> n^3" by simp
+      also assume "n^3 \<le> t n"
+      finally show "t n \<ge> n" .
+    qed
+
+    let ?T = "\<lambda>n. real (T n)"
+    from T_not_0 have *: "ae n. ?T n \<noteq> 0" by simp
+
+    with T_dominates_t' show "(\<lambda>n. t n * log 2 (t n) / T n) \<longlonglongrightarrow> 0"
+    proof (rule dominates_mono)
+      from t_min show "ae n. \<bar>t n * log 2 (t n)\<bar> \<le> \<bar>t' n * log 2 (t' n)\<bar>"
+      proof (ae_intro_nat)
+        fix n :: nat
+        assume "n \<ge> 2" and "n \<le> t n"
+        then have "t n \<ge> 2" by linarith
+
+        also have t_t': "t n \<le> t' n" unfolding l\<^sub>R_def t'_def comp_def
+          using \<open>mono t\<close> by (elim monoD) linarith
+        finally have "t' n \<ge> 2" .
+
+        with t_t' \<open>t n \<ge> 2\<close> have log_t_t': "log 2 (t n) \<le> log 2 (t' n)"
+          by (subst log_le_cancel_iff) linarith+
+
+        have "\<bar>f n * log 2 (f n)\<bar> = f n * log 2 (f n)" if "f n \<ge> 2" for f :: "nat \<Rightarrow> nat"
+          using that by force
+        note ** = this[of t, OF \<open>t n \<ge> 2\<close>] this[of t', OF \<open>t' n \<ge> 2\<close>]
+
+        from t_t' have "t n * log 2 (t n) \<le> t' n * log 2 (t n)"
+          using \<open>t n \<ge> 2\<close> by (intro mult_right_mono of_nat_mono) auto
+        also from log_t_t' have "... \<le> t' n * log 2 (t' n)"
+          using \<open>t n \<ge> 2\<close> by (intro mult_left_mono) linarith+
+        finally
+        show "\<bar>t n * log 2 (t n)\<bar> \<le> \<bar>t' n * log 2 (t' n)\<bar>" unfolding ** .
+      qed
+    qed
+  qed
+  then show "L\<^sub>0 \<in> DTIME(T) - DTIME(t)" and "dens L\<^sub>0 n \<le> dsqrt n"
+    unfolding L\<^sub>0_def by (fact lemma4_6.lemma4_6'')+
+qed
+
+thm_oracles lemma4_6 \<comment> \<open>shows \<open>skip_proof\<close> (the \<^emph>\<open>oracle\<close> used by \<open>sorry\<close>)\<close>
+
 
 end
